Causality example (#4)

aneris/examples/reliable_communication/examples/repdb_leader_followers/causality_example_proof.v
@@ -1,108 +1,33 @@
 From iris.algebra Require Import excl.
 From iris.base_logic.lib Require Import invariants.
+From aneris.prelude Require Import list.
 From aneris.aneris_lang Require Import ast.
 From aneris.aneris_lang.lib.serialization Require Import serialization_code.
 From aneris.aneris_lang Require Import lang.
-From aneris.aneris_lang Require Import tactics proofmode.
+From aneris.aneris_lang Require Import tactics proofmode adequacy.
 From aneris.aneris_lang.program_logic
-     Require Import aneris_weakestpre aneris_lifting.
+     Require Import aneris_weakestpre aneris_lifting aneris_adequacy.
 From aneris.aneris_lang.lib Require Import assert_proof.
 From aneris.aneris_lang.lib.serialization Require Import serialization_proof.
+From aneris.examples.reliable_communication.spec
+     Require Import prelude ras.
 From aneris.examples.reliable_communication.prelude
      Require Import ser_inj.
 From aneris.examples.reliable_communication.lib.repdb
-     Require Import repdb_code.
+     Require Import model repdb_code.
 From aneris.examples.reliable_communication.lib.repdb.spec
      Require Import ras events resources api_spec.
+From aneris.examples.reliable_communication.lib.repdb.proof
+     Require Import proof_of_db_init.
 From aneris.examples.reliable_communication.examples.repdb_leader_followers
      Require Import causality_example_code.
 From aneris.aneris_lang.program_logic Require Import lightweight_atomic.
-(*
-Section API_spec_ext.
-  Context `{!anerisG Mdl Σ, !DB_time, !DB_params, !DB_resources}.
-
-  Definition write_spec
-      (wr : val) (sa : socket_address) : iProp Σ :=
-    Eval simpl in
-    □ (∀ (E : coPset) (k : Key) (v : SerializableVal)
-         (P : iProp Σ) (Q : we → ghst → ghst → iProp Σ),
-        ⌜↑DB_InvName ⊆ E⌝ -∗
-        ⌜k ∈ DB_keys⌝ -∗
-        □ (P
-            ={⊤, E}=∗
-              ∃ (h : ghst) (a_old: option we),
-                ⌜at_key k h = a_old⌝ ∗
-                k ↦ₖ a_old ∗
-                Obs DB_addr h ∗
-                  ▷ (∀ (hf : ghst) (a_new : we),
-                  ⌜at_key k hf = None⌝ ∗
-                  ⌜we_key a_new = k⌝ ∗
-                  ⌜we_val a_new = v⌝ ∗
-                  ⌜∀ e, e ∈ h → e <ₜ a_new⌝ ∗
-                  k ↦ₖ Some a_new ∗
-                  Obs DB_addr (h ++ hf ++ [a_new]) ={E,⊤}=∗ Q a_new h hf)) -∗
-        {{{ P }}}
-          wr #k v @[ip_of_address sa]
-        {{{ RET #();
-           ∃ (h hf : ghst) (a: we), Q a h hf }}})%I.
-
-  Definition write_spec_atomic
-      (wr : val) (sa : socket_address) : iProp Σ :=
-    ∀ (E : coPset) (k : Key) (v : SerializableVal),
-    ⌜↑DB_InvName ⊆ E⌝ -∗
-    ⌜k ∈ DB_keys⌝ -∗
-    <<< ∀∀ (h : ghst) (a_old : option we),
-      ⌜at_key k h = a_old⌝ ∗
-      k ↦ₖ a_old ∗
-      Obs DB_addr h >>>
-      wr #k v @[ip_of_address sa] E
-    <<<▷ ∃∃ hf a_new, RET #();
-           ⌜at_key k hf = None⌝ ∗
-           ⌜we_key a_new = k⌝ ∗
-           ⌜we_val a_new = v⌝ ∗
-           ⌜∀ e, e ∈ h → e <ₜ a_new⌝ ∗
-           k ↦ₖ Some a_new ∗
-           Obs DB_addr (h ++ hf ++ [a_new]) >>>.
-
-  Lemma write_spec_write_spec_atomic wr sa :
-    write_spec wr sa -∗ write_spec_atomic wr sa.
-  Proof.
-    iIntros "#Hwr" (E k v HE Hkeys Φ) "!> Hvs".
-    iApply ("Hwr" $! E k v _ (λ _ _ _, Φ #()) with "[] [] [] Hvs");
-      [ done .. | | ].
-    { iIntros "!> Hvs".
-      iMod "Hvs" as (h a_old) "[(%Hatkey & Hk & Hobs) Hclose]".
-      iModIntro.
-      eauto 10 with iFrame. }
-    iIntros "!> H".
-    iDestruct "H" as (_ _ _) "H".
-    iApply "H".
-  Qed.
-
-  Axiom write_spec_implies_simplified_write_spec : ∀ wr sa,
-    write_spec wr sa -∗ ∀ k v h, simplified_write_spec wr sa k v h.
-
-  Definition read_spec_atomic (rd : val) (sa : socket_address) : iProp Σ :=
-    ∀ (E : coPset) (k : Key),
-    ⌜↑DB_InvName ⊆ E⌝ -∗
-    ⌜k ∈ DB_keys⌝ -∗
-    <<< ∀∀ (h : ghst) (q : Qp) (a_old : option we),
-            ⌜at_key k h = a_old⌝ ∗
-            Obs DB_addr h ∗
-            k ↦ₖ{q} a_old >>>
-      rd #k @[ip_of_address sa] E
-    <<<▷ RET match a_old with None => NONEV | Some a => SOMEV (we_val a) end;
-         (⌜a_old = None⌝ ∗ k ↦ₖ{q} None) ∨
-         (∃ e, ⌜a_old = Some e⌝ ∗
-            (k ↦ₖ{q} Some e)) >>>.
-
-End API_spec_ext.
 
 Section proof_of_code.
   Context `{!anerisG Mdl Σ}.
   Context `{TM: !DB_time, !DBPreG Σ}.
-  Context (leader_si : message → iProp Σ).
-  Context (db_sa db_Fsa : socket_address).
+  Context (leader_si follower_si : message → iProp Σ).
+  Context (db_l2csa db_f2csa db_l2fsa : socket_address).
 
   (* ------------------------------------------------------------------------ *)
   (** The definition of the parameters for DB and DL and shared resources. *)
@@ -110,8 +35,9 @@ Section proof_of_code.
 
   Local Instance DBSrv : DB_params :=
     {|
-      DB_addr := db_sa;
-      DB_addrF := db_Fsa;
+      DB_addr := db_l2csa;
+      DB_addrF := db_l2fsa;
+      DB_followers := {[db_f2csa]};
       DB_keys := {["x"; "y"]};
       DB_InvName := (nroot .@ "DBInv");
       DB_serialization := int_serialization;
@@ -121,159 +47,230 @@ Section proof_of_code.
 
   Context `{!@DB_resources _ _ _ _ DBSrv}.
 
-  Definition token (γ : gname) : iProp Σ := own γ (Excl ()).
+  Definition N := nroot.@"y".
 
-  Lemma token_exclusive (γ : gname) : token γ -∗ token γ -∗ False.
-  Proof. iIntros "H1 H2". by iDestruct (own_valid_2 with "H1 H2") as %?. Qed.
-
-  Definition Ny := nroot.@"y".
-  Definition Nx := nroot.@"x".
-
-  Definition inv_x (γ : gname) (a : we) : iProp Σ :=
-    ("x" ↦ₖ Some a ∗ ⌜we_val a = #37⌝) ∨ token γ.
-
-  Definition inv_y (γ : gname) : iProp Σ :=
-    ∃ h owe, Obs DB_addr h ∗ ⌜at_key "y" h = owe⌝ ∗ "y" ↦ₖ owe ∗
-             ∀ a, (⌜owe = Some a ∧ we_val a = (# 1)⌝) →
-                  (∃ a', ⌜a' <ₜ a⌝ ∗ inv Nx (inv_x γ a')).
-
-  (* TODO: Get empty history from nothing. *)
-  Lemma wp_do_writes wr clt_00 γ :
+  Lemma wp_wait_on_read clt_00 fsa rd h0:
     GlobalInv -∗
-    inv Ny (inv_y γ) -∗
+    (∀ k h, read_at_follower_spec rd clt_00 fsa k h) -∗
+    {{{ Obs fsa h0 }}}
+      wait_on_read rd #"y" #1 @[ip_of_address clt_00]
+    {{{ h' a, RET #();
+        ⌜h0 `prefix_of` h'⌝ ∗ Obs fsa h' ∗
+        ⌜(we_val a) = #1⌝ ∗ ⌜at_key "y" h' = Some a⌝ }}}.
+  Proof.
+    iIntros "#HGinv #Hard".
+    iIntros "!>" (Φ) "#HobsF HΦ".
+    wp_lam. wp_pures.
+    iLöb as "IH".
+    wp_apply ("Hard" $! "y" ); [done|done|]; iIntros (w).
+    iDestruct 1 as (h') "(%Hprefix & #HobsF' &
+                           [(-> & %Hatkey)|(%a & -> & %Hatkey)]) /=".
+    { wp_pures. iApply ("IH" with "HΦ"). }
+    wp_pures.
+    case_bool_decide as Ha.
+    { wp_pures. iApply "HΦ". by naive_solver. }
+    wp_pures. iApply ("IH" with "HΦ").
+  Qed.
+
+  Definition inv_def : iProp Σ :=
+    ("y" ↦ₖ None) ∨
+    (∃ h hfx hfy we_y we_x,
+        "y" ↦ₖ Some we_y ∗ "x" ↦ₖ Some we_x ∗
+        Obs db_l2csa (h ++ [we_x] ++ hfx ++ [we_y] ++ hfy) ∗
+        ⌜we_val we_x = #37⌝ ∗
+        ⌜at_key "x" h = None⌝ ∗ ⌜at_key "y" h = None⌝ ∗
+        ⌜at_key "x" hfx = None⌝ ∗ ⌜at_key "y" hfx = None⌝ ∗
+        ⌜at_key "x" hfy = None⌝ ∗ ⌜at_key "y" hfy = None⌝).
+
+  Lemma wp_do_writes wr clt_00 :
+    GlobalInv -∗
+    inv N inv_def -∗
     write_spec wr clt_00 -∗
-    Obs DB_addr [] -∗
+    Obs db_l2csa [] -∗
     {{{ "x" ↦ₖ None }}}
       do_writes wr @[ip_of_address clt_00]
     {{{ RET #(); True }}}.
   Proof.
     iIntros "#HGinv #Hinv #Hwr #Hobs".
     iIntros "!>" (Φ) "Hx HΦ".
-    iDestruct (write_spec_implies_simplified_write_spec with "Hwr") as "#Hswr".
+    iDestruct (get_simplified_write_spec with "Hwr") as "#Hswr".
     iDestruct (write_spec_write_spec_atomic with "Hwr") as "#Hawr".
     iClear "Hwr".
     wp_lam.
     wp_apply ("Hswr" $! _ (SerVal #37) with "[] [Hx]"); [done| |].
-    { iExists _. iFrame "#∗". done. }
+    { iExists _. by iFrame "#∗". }
     iDestruct 1 as (h a Hkey Hval Hatkey) "[#Hobs' Hx]".
     wp_pures.
-    iMod (inv_alloc Nx _ (inv_x γ a) with "[Hx]") as "#HIx".
-    { iModIntro. iLeft. eauto with iFrame. }
-    wp_apply ("Hawr" $! (⊤ ∖ ↑Ny) _ (SerVal #1)); [solve_ndisj|done|].
-    iInv Ny as "IH" "Hclose".
-    iDestruct "IH" as (h' owe) "(#>Hobs'' & >%Hatkey' & >Hy & _)".
-    iMod (Obs_compare with "HGinv Hobs' Hobs''") as %Hprefix; [solve_ndisj|].
-    iAssert (∃ hmax, ⌜(h ++ [a]) `prefix_of` hmax⌝ ∗
-                     ⌜h' `prefix_of` hmax⌝ ∗
-                     Obs DB_addr hmax)%I
-      as (hmax Hhmax1 Hhmax2) "Hobs'''".
-    { destruct Hprefix as [Hprefix | Hprefix].
-      - by iExists _; iFrame "Hobs''".
-      - by iExists _; iFrame "Hobs'". }
-    rewrite -Hatkey'.
-    iMod (OwnMemKey_obs_frame_prefix with "HGinv [$Hy $Hobs''']")
-      as "[Hy %Hatkey'']"; [solve_ndisj|done|].
-    rewrite Hatkey'.
+    wp_apply ("Hawr" $! (⊤ ∖ ↑N) _ (SerVal #1)); [solve_ndisj|done|].
+    iInv N as "IH" "Hclose".
+    iDestruct "IH" as "[>Hy | >IH]"; last first.
+    { iDestruct "IH" as (h' hfx hfy we_y we_x) "(Hy & Hx' & _)".
+      by iDestruct (OwnMemKey_exclusive with "Hx Hx'") as "[]". }
+    iMod (OwnMemKey_none_obs with "HGinv [$Hy $Hobs']") as "[Hy %Hhist]";
+      [solve_ndisj|].
+    assert (at_key "y" ([] ++ h ++ [a]) = None) as Hatkey'.
+    { rewrite /at_key. by rewrite Hhist. }
     iModIntro.
-    iExists hmax, owe.
-    rewrite -Hatkey''.
-    iFrame "#∗".
-    iSplit; [done|].
+    iExists ([] ++ h ++ [a]), None.
+    iFrame "#∗". iSplit; [done|].
     iNext.
     iIntros (h'' a').
-    iDestruct 1 as (Hatkey''' Hkey' Hval' Hle) "[Hy Hobs'''']".
-    simpl in *.
+    iDestruct 1 as (Hatkey''' Hkey' Hval' Hle) "[Hy #Hobs'']".
+    iMod (OwnMemKey_some_obs_frame with "HGinv [$Hx Hobs'']")
+      as "[Hx %Hatkey'''']"; [solve_ndisj| |].
+    { assert (([] ++ h ++ [a]) ++ h'' ++ [a'] =
+              (([] ++ h) ++ [a] ++ (h'' ++ [a']))) as ->;
+        [by rewrite !assoc|done]. }
+    assert (at_key "x" h'' = None).
+    { rewrite at_key_snoc_none in Hatkey''''; [done|by rewrite Hkey']. }
     iMod ("Hclose" with "[-HΦ]"); [|by iApply "HΦ"].
-    iNext.
-    iExists (hmax ++ h'' ++ [a']), (Some a'). iFrame.
-    iSplit; [|].
-    { iPureIntro.
-      rewrite /at_key !assoc hist_at_key_add_r_singleton; [|done].
-      apply last_snoc. }
-    iIntros (a'' [Heq Heq']).
-    simplify_eq.
-    iExists a.
-    iFrame "#".
-    iPureIntro.
-    apply Hle.
-    eapply elem_of_prefix; [|apply Hhmax1].
-    set_solver.
-  Qed.
-
-  Lemma wp_wait_on_read clt_00 clt_01 γ rd :
-    ip_of_address clt_00 = ip_of_address clt_01 →
-    GlobalInv -∗
-    read_spec_atomic rd clt_01 -∗
-    {{{ inv Ny (inv_y γ) }}}
-      wait_on_read rd #"y" #1 @[ip_of_address clt_00]
-    {{{ a, RET #(); inv Nx (inv_x γ a) }}}.
-  Proof.
-    iIntros (Hip) "#HGinv #Hard".
-    iIntros "!>" (Φ) "#Hinv HΦ".
-    wp_lam.
-    wp_pures.
-    iLöb as "IH".
-    wp_bind (rd _).
-    rewrite Hip.
-    wp_apply ("Hard" $! (⊤∖↑Ny)); [solve_ndisj|done|].
-    iInv Ny as "HI" "Hclose".
-    iDestruct "HI" as (h owe) "(#>Hobs & >%Hatkey & >Hy & #Himpl)".
-    iModIntro.
-    iExists h, _, owe.
+    iNext. iRight. iExists h, h'', [], a', a.
+    rewrite !app_assoc.
     iFrame "#∗".
-    iSplit; [done|].
-    iIntros "!> [H|H]".
-    { iDestruct "H" as (->) "Hy".
-      iMod ("Hclose" with "[-HΦ]").
-      { iIntros "!>". iExists _, _. iFrame "#∗". done. }
-      iModIntro.
-      wp_pures.
-      by iApply "IH". }
-    iDestruct "H" as (e ->) "Hy".
-    iMod ("Hclose" with "[-HΦ]").
-    { iIntros "!>". iExists _, _. iFrame "#∗". done. }
-    iModIntro.
-    wp_pures.
-    case_bool_decide as Heq.
-    - wp_pures.
-      iDestruct ("Himpl" with "[]") as (a) "[_ H]".
-      { by simplify_eq. }
-      by iApply "HΦ".
-    - wp_pures.
-      by iApply "IH".
+    rewrite hist_at_key_empty_at_key in Hhist.
+    rewrite at_key_snoc_none in Hhist; [done|by rewrite Hkey].
   Qed.
 
-  Lemma wp_do_reads clt_00 clt_01 γ rd :
-    ip_of_address clt_00 = ip_of_address clt_01 →
+  Lemma wp_do_reads clt_01 rd fsa :
     GlobalInv -∗
-    read_spec_atomic rd clt_01 -∗
-    inv Ny (inv_y γ) -∗
-    {{{ token γ }}}
-      do_reads rd @[ip_of_address clt_00]
+    (∀ k h, read_at_follower_spec rd clt_01 fsa k h) -∗
+    inv N inv_def -∗
+    Obs fsa [] -∗
+    {{{ True }}}
+      do_reads rd @[ip_of_address clt_01]
     {{{ RET #(); True }}}.
   Proof.
-    iIntros (Hip) "#HGinv #Hard #Hinvy".
-    iIntros "!>" (Φ) "Htok HΦ".
+    iIntros "#HGinv #Hard #Hinv_y #Hobs0".
+    iIntros "!>" (Φ) "_ HΦ".
     wp_lam.
     wp_apply (wp_wait_on_read); [done..|].
-    iIntros (a) "#Hinvx".
+    iIntros (h a) "(_ & #Hobs & _ & %Hatkey)".
     wp_pures.
-    rewrite Hip.
-    wp_apply ("Hard" $! (⊤∖↑Nx)); [solve_ndisj|done|].
-    iInv Nx as "HI" "Hclose".
-    iDestruct "HI" as "[>[Hx %Hval]|>HI]"; last first.
-    { iDestruct (token_exclusive with "Htok HI") as "[]". }
-    iMod (OwnMemKey_some_obs_we with "HGinv Hx") as "[Hx H]"; [solve_ndisj|].
-    iDestruct "H" as (h) "[#Hobs %Hatkey]".
-    iModIntro.
-    iExists _, _, _.
-    iFrame "#∗".
-    iSplit; [done|].
-    iIntros "!> [[%Heq _]|H]"; [done|].
-    iDestruct "H" as (e) "[%Heq Hx]".
-    simplify_eq.
-    iMod ("Hclose" with "[Htok]").
-    { by iRight. }
+    wp_apply ("Hard" $! "x"); [done..|].
+    iIntros (vo) "H".
+    iDestruct "H" as (h' Hprefix) "(#Hobs' & %Hdisj)".
+    iApply fupd_aneris_wp.
+    iInv N as "HI" "Hclose".
+    iDestruct "HI" as "[>Hy|>HI]".
+    { iMod (OwnMemKey_none_obs with "HGinv [$Hy $Hobs]")as "[Hy %Hhist]";
+        [solve_ndisj|].
+      by rewrite /at_key Hhist in Hatkey. }
+    iDestruct "HI" as (hb hfx hfy we_y we_x)
+                        "(Hy & Hx & #Hobs'' & %Hval &
+                        %Hatkey_hbx & %Hatkey_hby &
+                        %Hatkey_hfxx & %Hatkey_hfxy &
+                        %Hatkey_hfyx & %Hatkey_hfyy)".
+    iMod (OwnMemKey_key with "HGinv Hx") as "[Hx %Hkey_x]"; [solve_ndisj|].
+    iMod (OwnMemKey_key with "HGinv Hy") as "[Hy %Hkey_y]"; [solve_ndisj|].
+    assert (at_key "y" (hb ++ [we_x] ++ hfx ++ [we_y] ++ hfy) = Some we_y)
+           as Hatkey_y.
+    { rewrite /at_key.
+      rewrite hist_at_key_frame_l_prefix; [|done].
+      rewrite hist_at_key_frame_l_prefix; last first.
+      { rewrite /at_key /hist_at_key.
+        rewrite filter_cons_False; [done|by rewrite Hkey_x]. }
+      rewrite hist_at_key_frame_l_prefix; [|done].
+      rewrite hist_at_key_frame_r_suffix; [|done].
+      rewrite /at_key /hist_at_key.
+      rewrite filter_cons_True; [done|by rewrite Hkey_y]. }
+    assert (at_key "x" (hb ++ [we_x] ++ hfx ++ [we_y] ++ hfy) = Some we_x)
+           as Hatkey_x.
+    { rewrite /at_key.
+      rewrite hist_at_key_frame_l_prefix; [|done].
+      rewrite hist_at_key_frame_r_suffix.
+      { rewrite /at_key /hist_at_key.
+        rewrite filter_cons_True; [done|by rewrite Hkey_x]. }
+      rewrite /at_key.
+      rewrite hist_at_key_frame_l_prefix; [|done].
+      rewrite hist_at_key_frame_r_suffix; [|done].
+      rewrite /at_key /hist_at_key.
+      rewrite filter_cons_False; [done|by rewrite Hkey_y]. }
+    iAssert ("y" ↦ₖ Some we_y ={⊤ ∖ ↑N}=∗ ⌜a = we_y⌝ ∗ "y" ↦ₖ Some we_y)%I
+      as "H".
+    { iMod (Obs_compare with "HGinv Hobs Hobs''") as %Hprefix'; [solve_ndisj|].
+      iIntros "Hy".
+      destruct Hprefix' as [Hprefix'|Hprefix'].
+      - iModIntro. iFrame "Hy". iPureIntro.
+        rewrite !assoc in Hprefix'.
+        rewrite -assoc in Hprefix'.
+        eapply prefix_split_eq; [apply Hatkey| |done|apply Hprefix'].
+        rewrite !filter_app.
+        rewrite /at_key /hist_at_key !last_None in
+          Hatkey_hbx Hatkey_hby Hatkey_hfxx Hatkey_hfyx
+                     Hatkey_hfyy Hatkey_hfxy.
+        rewrite Hatkey_hby Hatkey_hfxy.
+        rewrite filter_cons_False; [done| by rewrite Hkey_x].
+      - rewrite -Hatkey_y.
+        iMod (OwnMemKey_obs_frame_prefix with "HGinv [$Hy $Hobs]")
+          as "[Hy %Heq]"; [solve_ndisj|done|].
+        rewrite -Heq in Hatkey.
+        rewrite Hatkey in Hatkey_y.
+        iModIntro.
+        iFrame "Hy".
+        iPureIntro.
+        by simplify_eq. }
+    iMod ("H" with "Hy") as (->) "Hy". iClear "H".
+    assert (∃ ao : option we,
+                at_key "x" h' = ao ∧
+                ((vo = InjLV #() ∧ ao = None) ∨
+                 (∃ a : we, vo = InjRV (we_val a) ∧ ao = Some a)))
+      as [a [Hatkey_a Hdisj']].
+    { destruct Hdisj as [Hdisj | Hdisj].
+      - destruct Hdisj as [-> Hdisj]. exists None. split; [done|by left].
+      - destruct Hdisj as [a [-> Hdisj]]. exists (Some a).
+        split; [done|by right;eexists _]. }
+    iAssert ("x" ↦ₖ Some we_x ={⊤ ∖ ↑N}=∗ ⌜a = Some we_x⌝ ∗ "x" ↦ₖ Some we_x)%I
+      as "H".
+    { iMod (Obs_compare with "HGinv Hobs' Hobs''") as %Hprefix'; [solve_ndisj|].
+      iIntros "Hx".
+      destruct Hprefix' as [Hprefix'|Hprefix'].
+      - iModIntro. iFrame "Hx". iPureIntro.
+        assert (h `prefix_of` hb ++ [we_x] ++ hfx ++ [we_y] ++ hfy) as Hprefix''.
+        { by eapply transitivity. }
+        rewrite !assoc in Hprefix''.
+        rewrite -assoc -assoc in Hprefix''.
+        assert (((hb ++ [we_x])) `prefix_of` h) as Hprefix'''.
+        { eapply prefix_Some_None.
+          - apply Hatkey.
+          - rewrite !filter_app.
+            rewrite /at_key /hist_at_key !last_None in
+              Hatkey_hbx Hatkey_hby Hatkey_hfxx Hatkey_hfyx
+                         Hatkey_hfyy Hatkey_hfxy.
+            rewrite Hatkey_hby.
+            rewrite filter_cons_False; [done|by rewrite Hkey_x].
+          - apply Hprefix''. }
+        destruct Hprefix''' as [k ->].
+        assert (∃ a', at_key "x" h' = Some a') as [a' Hatkey_a'].
+        { destruct Hprefix as [k' ->].
+          eapply (elem_of_last_filter_exists_Some _ _ a we_x).
+          - apply Hatkey_a.
+          - set_solver.
+          - done. }
+        assert (a = Some a') as -> by naive_solver.
+        f_equiv.
+        eapply prefix_split_eq; [apply Hatkey_a'|apply Hatkey_hbx| |apply Hprefix'].
+        + rewrite !filter_app.
+          rewrite /at_key /hist_at_key !last_None in
+            Hatkey_hbx Hatkey_hby Hatkey_hfxx Hatkey_hfyx
+                       Hatkey_hfyy Hatkey_hfxy.
+          rewrite Hatkey_hfxx Hatkey_hfyx.
+          rewrite filter_cons_False; [done|by rewrite Hkey_y].
+      - rewrite -Hatkey_x.
+        iMod (OwnMemKey_obs_frame_prefix with "HGinv [$Hx $Hobs']")
+          as "[Hy %Heq]"; [solve_ndisj|done|].
+        rewrite -Heq in Hatkey_a.
+        rewrite Hatkey_a in Hatkey_x.
+        iModIntro.
+        iFrame "Hy".
+        iPureIntro.
+        by simplify_eq. }
+    iMod ("H" with "Hx") as (->) "Hx". iClear "H".
+    destruct Hdisj' as [[_ Hineq]|Hdisj']; [done|].
+    destruct Hdisj' as [a [-> Heq]].
+    assert (we_x = a) as <-.
+    { by simplify_eq. }
+    iMod ("Hclose" with "[Hx Hy]") as "_".
+    { iRight. iExists _, _, _, _, _. by iFrame "Hx Hy #". }
     iModIntro.
     do 2 wp_pure _.
     wp_apply wp_assert.
@@ -283,5 +280,269 @@ Section proof_of_code.
     by iApply "HΦ".
   Qed.
 
+  Lemma proof_of_node0 (clt_00 : socket_address) A :
+    db_l2csa ∈ A →
+    clt_00 ∉ A →
+    GlobalInv -∗
+    fixed A -∗
+    (∀ A ca, init_client_proxy_leader_spec A ca leader_si) -∗
+    Obs db_l2csa [] -∗
+    inv N inv_def -∗
+    {{{ free_ports (ip_of_address clt_00) {[port_of_address clt_00]} ∗
+        clt_00 ⤳ (∅, ∅) ∗
+        db_l2csa ⤇ leader_si ∗
+        "x" ↦ₖ None }}}
+      node0 #clt_00 #db_l2csa @[ip_of_address clt_00]
+    {{{ RET #(); True }}}.
+  Proof.
+    iIntros (HIndb HnInA) "#HGinv #Hfixed #Hspec #Hobs #Hinv_y".
+    iIntros "!>" (Φ) "(Hfps & Hclt00 & #Hsi & Hx) HΦ".
+    wp_lam.
+    wp_pures.
+    wp_apply ("Hspec" with "[//] [//] [$Hfps $Hclt00]"); [by iFrame "#"|].
+    iIntros (wr rd) "[_ Hwr]".
+    wp_pures.
+    iApply (wp_do_writes with "[$] [$] [$] [$] Hx HΦ").
+  Qed.
+
+  Lemma proof_of_node1 (clt_01 : socket_address) A :
+    db_f2csa ∈ A →
+    clt_01 ∉ A →
+    GlobalInv -∗
+    fixed A -∗
+    (∀ A f2csa csa, init_client_proxy_follower_spec A csa f2csa follower_si) -∗
+    Obs db_f2csa [] -∗
+    inv N inv_def -∗
+    {{{ free_ports (ip_of_address clt_01) {[port_of_address clt_01]} ∗
+        clt_01 ⤳ (∅, ∅) ∗
+        db_f2csa ⤇ follower_si }}}
+      node1 #clt_01 #db_f2csa @[ip_of_address clt_01]
+    {{{ RET #(); True }}}.
+  Proof.
+    iIntros (HIndb HnInA) "#HGinv #Hfixed #Hspec #Hobs #Hinv_y".
+    iIntros "!>" (Φ) "(Hfps & Hclt00 & #Hsi) HΦ".
+    wp_lam.
+    wp_pures.
+    wp_apply ("Hspec" with "[//] [//] [$Hfps $Hclt00]"); [by iFrame "#"|].
+    iIntros (rd) "#Hrd".
+    wp_pures.
+    by iApply wp_do_reads.
+  Qed.
+
 End proof_of_code.
-*)
+
+(** Concrete parameters (addresses, ips) *)
+Definition db_l2csa := SocketAddressInet "0.0.0.0" 80.
+Definition db_l2fsa := SocketAddressInet "0.0.0.0" 81.
+Definition db_f2lsa := SocketAddressInet "0.0.0.1" 80.
+Definition db_f2csa := SocketAddressInet "0.0.0.1" 81.
+Definition clt_sa0 := SocketAddressInet "0.0.0.2" 80.
+Definition clt_sa1 := SocketAddressInet "0.0.0.3" 80.
+Definition A : gset socket_address := {[ db_l2csa; db_l2fsa; db_f2csa ]}.
+Definition ips : gset string := {[ "0.0.0.0" ; "0.0.0.1"; "0.0.0.2"; "0.0.0.3" ]}.
+Global Instance DBP : DB_params := DBSrv db_l2csa db_f2csa db_l2fsa.
+
+Definition main : expr :=
+    Start "0.0.0.0" (init_leader (DB_serialization.(s_serializer))
+                                 #db_l2csa #db_l2fsa);;
+    Start "0.0.0.1" (init_follower (DB_serialization.(s_serializer)) #db_l2fsa
+                                   #db_f2lsa #db_f2csa);;
+    Start "0.0.0.2" (node0 #clt_sa0 #db_l2csa);;
+    Start "0.0.0.3" (node1 #clt_sa1 #db_f2csa).
+
+
+Section proof_of_main.
+  Context `{!anerisG Mdl Σ, lockG Σ}.
+  Context `{TM: !DB_time, !DBPreG Σ}.
+  Context (leader_si leaderF_si follower_si : message → iProp Σ).
+  Context (InitL InitF : iProp Σ).
+  Context `{DBRes : !@DB_resources _ _ _ _ DBP}.
+
+  Lemma main_spec :
+    ⊢ |={⊤}=>
+         GlobalInv -∗
+         (∀ A, init_leader_spec A InitL leader_si leaderF_si) -∗
+         (∀ A csa, init_client_proxy_leader_spec A csa leader_si) -∗
+         (∀ A f2lsa, init_follower_spec f2lsa db_f2csa A InitF follower_si leaderF_si) -∗
+         (∀ A f2csa csa, init_client_proxy_follower_spec A csa f2csa follower_si) -∗
+         db_l2csa ⤇ leader_si -∗
+         db_l2fsa ⤇ leaderF_si -∗
+         db_f2csa ⤇ follower_si -∗
+         fixed A -∗
+         Obs db_l2csa [] -∗
+         Obs db_f2csa [] -∗
+         inv N (inv_def db_l2csa db_f2csa db_l2fsa) -∗
+         free_ip "0.0.0.0" -∗
+         free_ip "0.0.0.1" -∗
+         free_ip "0.0.0.2" -∗
+         free_ip "0.0.0.3" -∗
+         SocketAddressInet "0.0.0.0" 80 ⤳ (∅, ∅) -∗
+         SocketAddressInet "0.0.0.0" 81 ⤳ (∅, ∅) -∗
+         SocketAddressInet "0.0.0.1" 80 ⤳ (∅, ∅) -∗
+         SocketAddressInet "0.0.0.1" 81 ⤳ (∅, ∅) -∗
+         SocketAddressInet "0.0.0.2" 80 ⤳ (∅, ∅) -∗
+         SocketAddressInet "0.0.0.3" 80 ⤳ (∅, ∅) -∗
+         InitL -∗
+         InitF -∗
+         "x" ↦ₖ None -∗
+         WP main @["system"]
+      {{ v, True }}.
+  Proof.
+    iIntros "".
+    iModIntro.
+    iIntros "#HGinv #HdbSrvS #HdbCltS #HdbFS #HdbCltF".
+    iIntros "#Hdb_l2csa #Hdb_l2fsa #Hdb_f2csa #Hfixed #HobsL #HobsF #HI".
+    iIntros "Hfree0 Hfree1 Hfree2 Hfree3".
+    iIntros "Hsa0 Hsa1 Hsa2 Hsa3 Hsa4 Hsa5 HInitL HInitF".
+    iIntros "Hx".
+    rewrite /main.
+    wp_apply (aneris_wp_start {[80%positive; 81%positive]}); first done.
+    iFrame "Hfree0".
+    iSplitR "Hsa0 Hsa1 HInitL"; last first.
+    { iNext. iIntros "Hfps".
+      iApply ("HdbSrvS" $! A
+               with "[][][][][HInitL Hfps Hsa0 Hsa1]"); [eauto .. | | done ].
+      iDestruct (free_ports_split
+                    "0.0.0.0"
+                    {[80%positive]} {[81%positive]}) as "(Hfp1 & _)"; [set_solver|].
+      iFrame "#∗". iApply "Hfp1". iFrame. }
+    iNext. wp_pures.
+    wp_apply (aneris_wp_start {[80%positive;81%positive]}); first done.
+    iFrame "Hfree1".
+    iSplitR "Hsa2 Hsa3 HInitF"; last first.
+    { iNext. iIntros "Hfps".
+      iApply ("HdbFS" $! A db_f2lsa with "[//][//][][//][//][Hfps HInitF Hsa2 Hsa3]");
+        [iPureIntro; set_solver| |done].
+      iDestruct (free_ports_split
+                   "0.0.0.1"
+                   {[80%positive]} {[81%positive]} with "Hfps")
+        as "(Hfp1 & Hfp2)"; [set_solver|].
+      iFrame "#∗". }
+    iNext. wp_pures.
+    wp_apply (aneris_wp_start {[80%positive]}); first done.
+    iFrame "Hfree2".
+    iSplitR "Hsa4 Hx"; last first.
+    { iNext. iIntros "Hfps".
+      iApply (proof_of_node0 leader_si db_l2csa db_f2csa db_l2fsa clt_sa0 A
+               with "HGinv Hfixed HdbCltS HobsL HI [Hsa4 Hfps Hx]");
+        [done|set_solver| |done].
+      iFrame "#∗". }
+    iNext. wp_pures.
+    wp_apply (aneris_wp_start {[80%positive]}); first done.
+    iFrame "Hfree3".
+    iSplitR "Hsa5"; last first.
+    { iNext. iIntros "Hfps".
+      iApply (proof_of_node1 follower_si db_l2csa db_f2csa db_l2fsa clt_sa1 A
+               with "HGinv Hfixed HdbCltF HobsF HI [Hsa5 Hfps]");
+        [done|set_solver| |done].
+      iFrame "#∗". }
+    done.
+  Qed.
+
+End proof_of_main.
+
+Definition init_state :=
+  {|
+    state_heaps := {[ "system" := ∅ ]};
+    state_sockets := {[ "system" := ∅ ]};
+    state_ports_in_use :=
+      <["0.0.0.0" := ∅ ]> $
+      <["0.0.0.1" := ∅ ]> $
+      <["0.0.0.2" := ∅ ]> $
+      <["0.0.0.3" := ∅ ]> $ ∅;
+    state_ms := ∅;
+  |}.
+
+Definition dummy_model := model unit (fun x y => True) ().
+
+Lemma dummy_model_finitary : adequacy.aneris_model_rel_finitary dummy_model.
+Proof.
+  intros st.
+  intros f Hnot.
+  pose proof (Hnot 0%nat 1%nat) as H.
+  assert (0%nat = 1%nat -> False) as Himpl. {
+    intros Heq.
+    discriminate Heq.
+  }
+  apply Himpl; apply H.
+  destruct (f 0%nat) as [s0 r0].
+  destruct (f 1%nat) as [s1 r1].
+  destruct s0, s1, st, r0, r1.
+  reflexivity.
+Qed.
+
+Definition socket_interp `{!anerisG empty_model Σ}
+  db_l2csi db_l2fsi db_f2csi sa : socket_interp Σ :=
+  (match sa with
+   | SocketAddressInet "0.0.0.0" 80 => db_l2csi
+   | SocketAddressInet "0.0.0.0" 81 => db_l2fsi
+   | SocketAddressInet "0.0.0.1" 81 => db_f2csi
+   | _ => λ msg, ⌜True⌝
+   end)%I.
+
+Theorem adequacy : aneris_adequate main "system" init_state (λ _, True).
+Proof.
+  set (Σ := #[anerisΣ dummy_model; DBΣ; SpecChanΣ ]).
+  eapply (@adequacy
+            Σ dummy_model _ _ ips A
+            {[db_l2csa; db_l2fsa; db_f2lsa; db_f2csa; clt_sa0; clt_sa1]} ∅ ∅ ∅);
+    try done; last first.
+  { set_solver. }
+  { intros i. rewrite /ips !elem_of_union !elem_of_singleton.
+    intros [|]; subst; simpl; set_solver. }
+  { rewrite /ips /= !dom_insert_L dom_empty_L right_id_L //. set_solver. }
+  iIntros (Hdg) "".
+  2:{ apply dummy_model_finitary . }
+  assert (DBPreG Σ) as HPreG by apply _.
+  iMod (DB_init_setup ⊤ $! I) as (DBRes) "Hdb";
+    [solve_ndisj|set_solver|set_solver| ].
+  iDestruct "Hdb"
+    as (InitL leader_si leaderF_si) "(#HGinv & #Hobs & Hkeys & HInitL &
+                                      #[HinitL_spec HinitL_proxy_spec] &
+                                      HF)".
+  rewrite big_sepS_singleton.
+  iDestruct "HF" as (follower_si InitF) "(HInitF & #HobsF &
+                                          #HinitF_spec & #HinitF_proxy_spec)".
+  iExists (socket_interp leader_si leaderF_si follower_si).
+  iMod (@main_spec
+          _ _ _
+          int_time leader_si leaderF_si follower_si InitL InitF DBRes) as "Hmain".
+  iModIntro.
+  iIntros "Hf Hsis Hb Hfg Hips _ _ _ _ _".
+  iDestruct (big_sepS_delete _ _ db_l2csa with "Hsis") as "[Hsi0 Hsis]";
+    first set_solver.
+  iDestruct (big_sepS_delete _ _ db_l2fsa with "Hsis") as "[Hsi1 Hsis]";
+    first set_solver.
+  iDestruct (big_sepS_delete _ _ db_f2csa with "Hsis") as "[Hsi2 _]";
+    first set_solver.
+  iDestruct (big_sepS_delete _ _ "0.0.0.0" with "Hips") as "[Hip0 Hips]";
+    first set_solver.
+  iDestruct (big_sepS_delete _ _ "0.0.0.1" with "Hips") as "[Hip1 Hips]";
+    first set_solver.
+  iDestruct (big_sepS_delete _ _ "0.0.0.2" with "Hips") as "[Hip2 Hips]";
+    first set_solver.
+  iDestruct (big_sepS_delete _ _ "0.0.0.3" with "Hips") as "[Hip3 Hips]";
+    first set_solver.
+  iDestruct (big_sepS_delete _ _ db_l2csa with "Hb") as "[Hm0 Hms]";
+    first set_solver.
+  iDestruct (big_sepS_delete _ _ db_l2fsa with "Hms") as "[Hm1 Hms]";
+    first set_solver.
+  iDestruct (big_sepS_delete _ _ db_f2lsa with "Hms") as "[Hm2 Hms]";
+    first set_solver.
+  iDestruct (big_sepS_delete _ _ db_f2csa with "Hms") as "[Hm3 Hms]";
+    first set_solver.
+  iDestruct (big_sepS_delete _ _ clt_sa0 with "Hms") as "[Hc0 Hms]";
+    first set_solver.
+  iDestruct (big_sepS_delete _ _ clt_sa1 with "Hms") as "[Hc1 Hms]";
+    first set_solver.
+  iDestruct (big_sepS_delete _ _ "x" with "Hkeys") as "[Hx Hkeys]";
+    first set_solver.
+  iDestruct (big_sepS_delete _ _ "y" with "Hkeys") as "[Hy _]";
+   first set_solver.
+  iMod (inv_alloc N _ (inv_def db_l2csa db_f2csa db_l2fsa) with "[Hy]") as "HI".
+  { by iLeft. }
+  iApply ("Hmain" with
+           "HGinv HinitL_spec HinitL_proxy_spec HinitF_spec HinitF_proxy_spec
+            Hsi0 Hsi1 Hsi2 Hf Hobs HobsF HI Hip0 Hip1 Hip2 Hip3
+            Hm0 Hm1 Hm2 Hm3 Hc0 Hc1 HInitL HInitF Hx").
+Qed.
